preliminary fx10 impl

FX10.v
@@ -1,73 +1,120 @@
 (** Featherweight X10 Implementation *)
 
-Definition array := list nat.
-Notation "x :: l" := (cons x l)
-                     (at level 60, right associativity).
-Notation "[ ]" := nil.
-Notation "[ x ; .. ; y ]" := (cons x .. (cons y nil) ..).
+From LF Require Export Array.
+From LF Require Export Syntax.
 
-Fixpoint access (A : array) (index : nat) : nat :=
-  match index with
-  | O => match A with
-    | nil => O
-    | h :: t => h
-  end
-  | S index' => match A with
-    | nil => O
-    | h :: t => access t index'
-  end
-end.
-
-Example test_access0:  (access [1; 2; 3] 0) = 1.
-Proof. simpl. reflexivity.  Qed.
-Example test_access1:  (access [1; 2; 3] 1) = 2.
-Proof. simpl. reflexivity.  Qed.
-Example test_access2:  (access [1; 2; 3] 2) = 3.
-Proof. simpl. reflexivity.  Qed.
-Example test_access3:  (access [1; 2; 3] 3) = 0.
-Proof. simpl. reflexivity.  Qed.
-
-Fixpoint insert (A : array) (index : nat) (value : nat) : array := 
-  match index with
-  | O => match A with
-    | nil => value :: nil
-    | h :: t => value :: t
-  end
-  | S index' => match A with
-    | nil => value :: nil
-    | h :: t => h :: insert t index' value
-  end
-end.
-
-Example test_insert0:  (insert [1; 1; 1] 0 2) = [2; 1; 1].
-Proof. simpl. reflexivity.  Qed.
-Example test_insert1:  (insert [1; 1; 1] 1 2) = [1; 2; 1].
-Proof. simpl. reflexivity.  Qed.
-Example test_insert2:  (insert [1; 1; 1] 2 2) = [1; 1; 2].
-Proof. simpl. reflexivity.  Qed.
-Example test_insert3:  (insert [1; 1; 1] 3 2) = [1; 1; 1; 2].
-Proof. simpl. reflexivity.  Qed.
-
-
-
-Inductive statement : Type :=
-| skip : statement
-| seq (i : instr) (s : statement) : statement
+Inductive tree : Type :=
+| done : tree
+| statements (s : statement) : tree
+| arrow (T1 : tree) (T2 : tree) : tree
+| pipes (T1 : tree) (T2 : tree) : tree
 .
 
-Definition instr : Type :=
-| skip : instr
-(* a[d] = e *)
-(* while (a[d] != 0) s *)
-| async (s : statement) : instr
-| finish (s : statement) : instr
-| call
+Notation "x || y" := (pipes x y).
+Notation "x :> y" := (arrow x y) (at level 62).
+
+Inductive State := | state (p : program) (A : array) (T : tree).
+
+Inductive stepsto : State -> State -> Prop :=
+| stepsto_1 (p : program) (A : array) (T : tree):
+    stepsto 
+      (state p A (done :> T)) 
+      (state p A T)
+| stepsto_2 (p : program) (A : array) (T : tree) (A' : array) (T' : tree) (T2 : tree):
+    stepsto 
+      (state p A T) 
+      (state p A' T') 
+    -> 
+    stepsto 
+      (state p A (T :> T2)) 
+      (state p A' (T' :> T2))
+| stepsto_3 (p : program) (A : array) (T : tree):
+    stepsto 
+      (state p A (done || T)) 
+      (state p A T)
+| stepsto_4 (p : program) (A : array) (T : tree):
+    stepsto 
+      (state p A (T || done)) 
+      (state p A T)
+| stepsto_5 (p : program) (A : array) (T : tree) (A' : array) (T' : tree) (T2 : tree):
+    stepsto 
+      (state p A T) 
+      (state p A' T') 
+    -> 
+    stepsto 
+      (state p A (T || T2)) 
+      (state p A' (T' || T2))
+| stepsto_6 (p : program) (A : array) (T : tree) (A' : array) (T' : tree) (T2 : tree):
+    stepsto 
+      (state p A T) 
+      (state p A' T') 
+    -> 
+    stepsto 
+      (state p A (T2 || T)) 
+      (state p A' (T2 || T'))
+| stepsto_7 (p : program) (A : array):
+    stepsto 
+      (state p A (statements skip)) 
+      (state p A done)
+| stepsto_8 (p : program) (A : array) (k : statement):
+    stepsto 
+      (state p A (statements (seq skp k))) 
+      (state p A (statements k))
+| stepsto_9 (p : program) (A : array) (k : statement) (d : nat) (e : expr):
+    stepsto 
+      (state p A (statements (seq (assignment A d e) k))) 
+      (
+        match e with 
+        | const n => (state p (assign A d n) (statements k))
+        | incr a i => (state p (assign A d (access A i)) (statements k))
+        end
+      )
+| stepsto_10_11 (p : program) (A : array) (k : statement) (d : nat) (s : statement):
+    stepsto 
+      (state p A (statements (seq (while A d s) k))) 
+      (
+        match (access A d) with 
+        | O => (state p A (statements k))
+        | S n => (state p A (statements (join s (seq (while A d s) k))))
+        end
+      )
+| stepsto_12 (p : program) (A : array) (k : statement) (s : statement):
+    stepsto 
+      (state p A (statements (seq (async s) k)))
+      (state p A ((statements s) || (statements k)))
+| stepsto_13 (p : program) (A : array) (k : statement) (s : statement):
+    stepsto 
+      (state p A (statements (seq (finish s) k)))
+      (state p A ((statements s) :> (statements k)))
+| stepsto_14 (p : program) (A : array) (k : statement) (s : statement):
+    stepsto 
+      (state p A (statements (seq (call s) k)))
+      (state p A (statements (join s k)))
 .
 
-Definition expr : Type := 
-| nat : expr
-(* a[d] + 1 *)
-.
-
-
-
+Example test_stepsto1:  
+  stepsto 
+    (state (p {}) (array_init 0) (done :> (statements {skp}))) 
+    (state (p {}) (array_init 0) (statements {skp})).
+Proof. apply stepsto_1. Qed.
+(* TODO Example test_stepsto2: *)
+Example test_stepsto3:  
+  stepsto 
+    (state (p {}) (array_init 0) (done || (statements {skp}))) 
+    (state (p {}) (array_init 0) (statements {skp})).
+Proof. apply stepsto_3. Qed.
+Example test_stepsto4:  
+  stepsto 
+    (state (p {}) (array_init 0) ((statements {skp}) || done))
+    (state (p {}) (array_init 0) (statements {skp})).
+Proof. apply stepsto_4. Qed.
+(* TODO Example test_stepsto5: *)
+(* TODO Example test_stepsto6: *)
+(* TODO Example test_stepsto7: *)
+(* TODO Example test_stepsto8: *)
+(* TODO Example test_stepsto9: *)
+(* TODO Example test_stepsto10: *)
+(* TODO Example test_stepsto11: *)
+(* TODO Example test_stepsto12: *)
+(* TODO Example test_stepsto13: *)
+(* TODO Example test_stepsto14: *)
