Array.v
@@ -1,0 +1,63 @@
+Definition array : Type := list nat.
+Notation "x :: l" := (cons x l)
+                     (at level 60, right associativity).
+Notation "[ ]" := nil.
+Notation "[ x ; .. ; y ]" := (cons x .. (cons y nil) ..).
+
+Fixpoint access (A : array) (index : nat) : nat :=
+  match index with
+  | O => match A with
+    | nil => O
+    | h :: t => h
+  end
+  | S index' => match A with
+    | nil => O
+    | h :: t => access t index'
+  end
+end.
+
+Example test_access0:  (access [1; 2; 3] 0) = 1.
+Proof. simpl. reflexivity.  Qed.
+Example test_access1:  (access [1; 2; 3] 1) = 2.
+Proof. simpl. reflexivity.  Qed.
+Example test_access2:  (access [1; 2; 3] 2) = 3.
+Proof. simpl. reflexivity.  Qed.
+Example test_access3:  (access [1; 2; 3] 3) = 0.
+Proof. simpl. reflexivity.  Qed.
+
+Fixpoint assign (A : array) (index : nat) (value : nat) : array := 
+  match index with
+  | O => match A with
+    | nil => nil
+    | h :: t => value :: t
+  end
+  | S index' => match A with
+    | nil => nil
+    | h :: t => h :: assign t index' value
+  end
+end.
+
+Example test_assign0:  (assign [1; 1; 1] 0 2) = [2; 1; 1].
+Proof. simpl. reflexivity.  Qed.
+Example test_assign1:  (assign [1; 1; 1] 1 2) = [1; 2; 1].
+Proof. simpl. reflexivity.  Qed.
+Example test_assign2:  (assign [1; 1; 1] 2 2) = [1; 1; 2].
+Proof. simpl. reflexivity.  Qed.
+Example test_assign3:  (assign [1; 1; 1] 3 2) = [1; 1; 1].
+Proof. simpl. reflexivity.  Qed.
+Example test_assign4:  (assign [1; 1; 1] 4 2) = [1; 1; 1].
+Proof. simpl. reflexivity.  Qed.
+
+Fixpoint array_init (size : nat) : array :=
+  match size with
+  | O => nil
+  | S n => O :: array_init n
+  end
+.
+
+Example test_array_init0:  array_init O = [].
+Proof. simpl. reflexivity.  Qed.
+Example test_array_init1:  array_init 1 = [0].
+Proof. simpl. reflexivity.  Qed.
+Example test_array_init2:  array_init 2 = [0; 0].
+Proof. simpl. reflexivity.  Qed.
