DeadlockFreedom.v
@@ -1,0 +1,20 @@
+(* Deadlock Freedom Proof *)
+
+From LF Require Export FX10.
+
+Inductive isComplete : State -> Prop :=
+| doneTree (p : program) (A : array) :
+    isComplete (state p A done)
+.
+
+Theorem isCompleteCheck : forall (p : program) (A : array),
+  isComplete (state p A done).
+Proof.
+  - intros p A. apply doneTree.
+Qed.
+
+Theorem deadlock_freedom_fx10 : forall S : State,
+  isComplete S \/ exists S', stepsto S S'.
+Proof.
+  Admitted.
+(* TODO *)
