Syntax.v
@@ -1,0 +1,55 @@
+
+From LF Require Export Array.
+
+Inductive expr : Type := 
+| const (n : nat) : expr
+| incr (A : array) (index : nat) : expr
+.
+
+Inductive sequence (X : Type) : Type :=
+| skip
+| seq (x : X) (l : sequence X)
+.
+Arguments skip {X}.
+Arguments seq {X} _ _.
+
+Inductive instr : Type :=
+| skp : instr  (* Handled in statement so unnecessary *)
+| assignment (A : array) (index : nat) (e : expr) : instr
+| while (A : array) (index : nat) (s : sequence instr) : instr
+| async (s : sequence instr) : instr
+| finish (s : sequence instr) : instr
+| call (s : sequence instr) : instr
+.
+
+(* 
+Notation "a [ d ] = e" := (assignment a d e) (at level 64).
+Notation "while ( a [ d ] ! 0 ) s" := (while a d s) (at level 64).
+*)
+
+Definition statement : Type := sequence instr.
+Notation "x >> l" := (seq x l)
+                     (at level 61, right associativity).
+Notation "{ }" := skip.
+Notation "{ x ; .. ; y }" := (seq x .. (seq y skip) ..).
+
+Fixpoint join (s1 : statement) (s2 : statement) : statement :=
+match s1 with 
+| skip => s2
+| seq i s => i >> (join s s2)
+end.
+
+Example test_join:  join {skp; skp; call {skp}} {skp; skp} = {skp; skp; call {skp}; skp; skp}.
+Proof. simpl. reflexivity. Qed.
+
+Inductive program : Type := 
+| p (s : statement) : program
+.
+
+Check p ({ }).
+Check p ({skp}).
+Check p ({skp; skp}).
+Check p ({skp; skp; async {skp}}).
+Check p ({skp; skp; finish {async {skp}}}).
+Check p ({finish {async {skp}}; while [1] 0 {assignment [5] 0 (const 1)}}).
+Check p ({call {skp; call {skp; assignment [3; 5] 1 (incr [2] 0)}; skp; call {skp}}}).
